0421 Prooved preservation in System F

plc/PLC.v
@@ -1,14 +1,6 @@
-From Stdlib Require Import Bool.
-From Stdlib Require Import Init.Nat.
-From Stdlib Require Import Arith.
-From Stdlib Require Import EqNat. Import Nat.
-From Stdlib Require Import Lia.
-From Stdlib Require Import List. Import ListNotations.
-From Stdlib Require Import Strings.String.
-From Stdlib Require Import Program.Equality.
 From Stdlib Require Import FunctionalExtensionality.
 
-From PLC Require Import Maps.
+From PLC Require Export Maps.
 
 (** * Polymorphic lambda calculus *)
 
@@ -79,9 +71,6 @@ Hint Unfold z : core.
 Hint Unfold X : core.
 Hint Unfold Y : core.
 Hint Unfold Z : core.
-
-Check <{ \\ X , unit }>.
-(* Check <{{ (Bool -> Bool) -> Bool }}>. *)
 
 Reserved Notation "'[' x ':=' s ']' t" (in custom plc_tm at level 5, x global, s custom plc_tm,
       t custom plc_tm at next level, right associativity).
@@ -177,48 +166,6 @@ Inductive multi {X:Type} (R: X -> X -> Prop) : X -> X -> Prop :=
 Notation multistep := (multi step).
 Notation "t1 '-->*' t2" := (multistep t1 t2) (at level 40).
 
-(* Examples *)
-  Example step_appabs_example :
-    <{ (\x:Unit, x) unit }> --> <{ unit }>.
-  Proof.
-    apply ST_AppAbs.
-    constructor.
-  Qed.
-
-  Example step_app1_example :
-    <{ ((\x:Unit, x) unit) unit }> --> <{ (unit) unit }>.
-  Proof.
-    apply ST_App1.
-    apply ST_AppAbs.
-    constructor.
-  Qed.
-
-  Example step_app2_example :
-    <{ (\x:Unit, x) ((\x:Unit, x) unit) }> --> <{ (\x:Unit, x) unit }>.
-  Proof.
-    apply ST_App2.
-    - constructor.
-    - apply ST_AppAbs.
-      constructor.
-  Qed.
-
-  Example step_tappabs_example :
-    <{ (\\X, \x: X, x) [Unit] unit }> -->* <{ unit }>.
-  Proof.
-    eapply multi_step.
-    - apply ST_App1. apply ST_TAppAbs.
-    - simpl. eapply multi_step.
-      + apply ST_AppAbs. constructor.
-      + simpl. apply multi_refl. 
-  Qed.
-
-  Example step_tapp_example :
-    <{ ((\\X, unit) [Unit]) [Unit] }> --> <{ (unit) [Unit] }>.
-  Proof.
-    apply ST_TApp.
-    apply ST_TAppAbs.
-  Qed.
-
 Definition context := partial_map ty.
 
 Notation "x '|->' v ';' m " := (update m x v)
@@ -302,71 +249,176 @@ Proof.
 Qed.
 
 (* Preservation *)
-Lemma weakening : forall Gamma Gamma' t T,
-     includedin Gamma Gamma' ->
-     <{ Gamma  |-- t \in T }>  ->
-     <{ Gamma' |-- t \in T }>.
-Proof.
-  intros Gamma Gamma' t T H Ht.
-  generalize dependent Gamma'.
-  induction Ht; intros; econstructor.
-  - apply H0. assumption.
-  - apply IHHt. apply includedin_update. apply H.
-  - apply IHHt1. assumption.
-  - apply IHHt2. assumption.
-  - apply IHHt. assumption.
-  - apply H.
-  - apply IHHt. assumption.
-Qed.
+(* Variables *)
+Inductive var_appears_free_in (x : string) : tm -> Prop :=
+  | vaf_var : var_appears_free_in x <{x}>
+  | vaf_app1 : forall t1 t2,
+      var_appears_free_in x t1 ->
+      var_appears_free_in x <{t1 t2}>
+  | vaf_app2 : forall t1 t2,
+      var_appears_free_in x t2 ->
+      var_appears_free_in x <{t1 t2}>
+  | vaf_abs : forall y T1 t1,
+      y <> x  ->
+      var_appears_free_in x t1 ->
+      var_appears_free_in x <{\y:T1, t1}>
+  | vaf_tyapp : forall t T,
+      var_appears_free_in x t ->
+      var_appears_free_in x <{t[T]}>
+  | vaf_tyabs : forall X t,
+      var_appears_free_in x t ->
+      var_appears_free_in x <{\\X, t}>.
+Hint Constructors var_appears_free_in : core.
 
-Lemma weakening_empty : forall Gamma t T,
-     <{ empty |-- t \in T }> ->
-     <{ Gamma |-- t \in T }>.
-Proof.
-  intros Gamma t T.
-  eapply weakening.
-  unfold includedin. intros. discriminate.
-Qed.
+Inductive not_var_appears_free_in (x : string) : tm -> Prop :=
+  | nvaf_var : forall (y: string),
+      y <> x ->
+      not_var_appears_free_in x <{y}>
+  | nvaf_app : forall t1 t2,
+      not_var_appears_free_in x t1 ->
+      not_var_appears_free_in x t2 ->
+      not_var_appears_free_in x <{t1 t2}>
+  | nvaf_abs1 : forall T1 t1,
+      not_var_appears_free_in x <{\x:T1, t1}>
+  | nvaf_abs2 : forall y T1 t1,
+      y <> x ->
+      not_var_appears_free_in x t1 ->
+      not_var_appears_free_in x <{\y:T1, t1}>
+  | nvaf_tyapp : forall t T,
+      not_var_appears_free_in x t ->
+      not_var_appears_free_in x <{t[T]}>
+  | nvaf_tyabs : forall X t,
+      not_var_appears_free_in x t ->
+      not_var_appears_free_in x <{\\X, t}>
+  | nvaf_unit :
+      not_var_appears_free_in x <{unit}>.
+Hint Constructors not_var_appears_free_in : core.
 
-Lemma type_preservation_subst: forall Gamma x s S t T,
-  <{ x |-> S; Gamma |-- t \in T }> ->
-  <{ empty |-- s \in S }> ->
-  <{ Gamma |-- [x:=s] t \in T }>.
+Lemma notvaf_nvaf_iff : forall x t,
+  ~ var_appears_free_in x t <-> not_var_appears_free_in x t.
 Proof.
-  intros Gamma x s S t T Ht Hs.
-  remember (x |-> S; Gamma) as Gamma'.
-  generalize dependent Gamma.
-  induction Ht; simpl; intros; subst.
-  - unfold update in H. unfold t_update in H.
-    destruct (x=?x0)%string eqn: Eqx.
-    + inversion H. subst. apply weakening_empty.
+  intros x t. split; intro H.
+  - induction t.
+    + constructor. intros contra. subst. apply H. constructor.
+    + destruct (x=?x0)%string eqn: Eqx.
+      * rewrite eqb_eq in Eqx. subst. constructor. 
+      * constructor.
+        { apply eqb_neq. rewrite eqb_sym. assumption. }
+        { apply IHt. intro contra. apply H. constructor.
+          - apply eqb_neq. rewrite eqb_sym. assumption.
+          - assumption. }
+    + constructor; [apply IHt1| apply IHt2]; 
+      intro Hvaf; apply H; [apply vaf_app1 | apply vaf_app2];
       assumption.
-    + apply T_Var. apply H.
-  - destruct (x=?x0)%string eqn: Eqx.
-    + apply T_Abs.
-      apply weakening with (Gamma:=x0 |-> T2; x |-> S; Gamma0).
-      * unfold includedin. intros.
-        apply eqb_eq in Eqx. subst x.
-        rewrite <- update_shadow with (v1:=S). apply H.
-      * apply Ht.
-    + apply T_Abs. apply IHHt.
-      apply update_permute. apply eqb_neq. apply Eqx.
-  - eapply T_App.
-    * apply IHHt1. reflexivity.
-    * apply IHHt2. reflexivity.
-  - apply T_TAbs. apply IHHt. reflexivity.
-  - apply T_TApp with (X:=X0) (T1:=T1).
-    * reflexivity.
-    * apply IHHt. reflexivity.
-  - apply T_Unit.
+    + constructor. apply IHt. intro Hvaf. apply H.
+      constructor. assumption.
+    + constructor. apply IHt. intro Hvaf. apply H.
+      constructor. assumption.
+    + constructor.    
+  - intro contra. induction contra; inversion H; subst; auto.
 Qed.
 
-Definition context_ty_subst X S (Gamma: context) : context :=
-    fun x =>
-      match Gamma x with
-      | Some T => Some (<{{[X:=S] T}}>)
-      | None => None
-      end.
+Inductive var_appears_bounded_in (x : string) : tm -> Prop :=
+  | vab_app1 : forall t1 t2,
+      var_appears_bounded_in x t1 ->
+      var_appears_bounded_in x <{t1 t2}>
+  | vab_app2 : forall t1 t2,
+      var_appears_bounded_in x t2 ->
+      var_appears_bounded_in x <{t1 t2}>
+  | vab_abs1 : forall T1 t1,
+      var_appears_bounded_in x <{\x:T1, t1}>
+  | vab_abs2 : forall y T1 t1,
+      y <> x ->
+      var_appears_bounded_in x t1 ->
+      var_appears_bounded_in x <{\y:T1, t1}>
+  | vab_tyabs : forall X t,
+      var_appears_bounded_in x t ->
+      var_appears_bounded_in x <{\\X, t}>
+  | vab_tyapp : forall t T,
+      var_appears_bounded_in x t ->
+      var_appears_bounded_in x <{t[T]}>.
+Hint Constructors var_appears_bounded_in : core.
+
+Inductive not_var_appears_bounded_in (x : string) : tm -> Prop :=
+  | nvab_var : forall (y: string),
+      not_var_appears_bounded_in x <{y}>
+  | nvab_app : forall t1 t2,
+      not_var_appears_bounded_in x t1 ->
+      not_var_appears_bounded_in x t2 ->
+      not_var_appears_bounded_in x <{t1 t2}>
+  | nvab_abs : forall y T1 t1,
+      y <> x ->
+      not_var_appears_bounded_in x t1 ->
+      not_var_appears_bounded_in x <{\y:T1, t1}>
+  | nvab_tyabs : forall X t,
+      not_var_appears_bounded_in x t ->
+      not_var_appears_bounded_in x <{\\X, t}>
+  | nvab_tyapp : forall t T,
+      not_var_appears_bounded_in x t ->
+      not_var_appears_bounded_in x <{t[T]}>
+  | nvab_unit :
+      not_var_appears_bounded_in x <{unit}>.
+Hint Constructors not_var_appears_bounded_in : core.
+
+Lemma notvab_nvab_iff : forall x t,
+  ~ var_appears_bounded_in x t <-> not_var_appears_bounded_in x t.
+Proof.
+  intros x t. split; intro H.
+  - induction t.
+    + constructor.
+    + destruct (x =? x0)%string eqn:Heq.
+      * rewrite String.eqb_eq in Heq. subst. exfalso.
+        apply H. constructor.
+      * apply nvab_abs.
+        -- intro contra. subst. rewrite String.eqb_refl in Heq. discriminate.
+        -- apply IHt. intro contra. apply H. apply vab_abs2; auto.
+            intro contra2. subst. rewrite String.eqb_refl in Heq. discriminate.
+    + constructor; [apply IHt1|apply IHt2]; intro contra; apply H; eauto.
+    + constructor. apply IHt. intro Hvab. apply H.
+      constructor. assumption.
+    + constructor. apply IHt. intro Hvab. apply H.
+      constructor. assumption.
+    + constructor. 
+  - intro contra. induction contra; inversion H; subst; auto.
+Qed.
+
+Inductive var_bounded_left_notfree_right : tm -> Prop :=
+  | vblnfr_var : forall (x: string),
+      var_bounded_left_notfree_right <{x}>
+  | vblnfr_abs : forall x T1 t1,
+      var_bounded_left_notfree_right t1 ->
+      var_bounded_left_notfree_right <{\x:T1, t1}>
+  | vblnfr_app : forall t1 t2,
+      ( forall x,
+        var_appears_free_in x t2 ->
+        ~ var_appears_bounded_in x t1 ) ->
+      var_bounded_left_notfree_right t1 ->
+      var_bounded_left_notfree_right t2 ->
+      var_bounded_left_notfree_right <{t1 t2}>
+  | vblnfr_tyabs : forall X t,
+      var_bounded_left_notfree_right t ->
+      var_bounded_left_notfree_right <{\\X, t}>
+  | vblnfr_tyapp : forall t T,
+      var_bounded_left_notfree_right t ->
+      var_bounded_left_notfree_right <{t[T]}>
+  | vblnfr_unit :
+      var_bounded_left_notfree_right <{unit}>.
+Hint Constructors var_bounded_left_notfree_right : core.
+
+(* Type Variables *)
+Inductive tyvar_appears_free_in_ty (X: string) : ty -> Prop :=
+  | tvaf_var :
+      tyvar_appears_free_in_ty X (TyVar X)
+  | tvaf_arrow1 : forall T1 T2,
+      tyvar_appears_free_in_ty X T1 ->
+      tyvar_appears_free_in_ty X <{{T1 -> T2}}>
+  | tvaf_arrow2 : forall T1 T2,
+      tyvar_appears_free_in_ty X T2 ->
+      tyvar_appears_free_in_ty X <{{T1 -> T2}}>
+  | tvaf_forall : forall Y T1,
+      X <> Y ->
+      tyvar_appears_free_in_ty X T1 ->
+      tyvar_appears_free_in_ty X <{{-/Y, T1}}>.
 
 Inductive not_tyvar_appears_free_in_ty (X: string) : ty -> Prop :=
   | ntvaf_var : forall Y,
@@ -385,47 +437,175 @@ Inductive not_tyvar_appears_free_in_ty (X: string) : ty -> Prop :=
   | ntvaf_unit :
       not_tyvar_appears_free_in_ty X <{{Unit}}>.
 
-Definition closed T :=
-  forall X, not_tyvar_appears_free_in_ty X T.
-
-Lemma ntvaf_subst_ty : forall X S T,
-  not_tyvar_appears_free_in_ty X T ->
-  T = <{{ [X:=S] T }}>.
+Lemma nottvaf_ntvaf_iff : forall X T,
+  ~ tyvar_appears_free_in_ty X T <-> not_tyvar_appears_free_in_ty X T.
 Proof.
-  intros. induction H; simpl;
-  try rewrite eqb_refl;
-  try (apply eqb_neq in H; rewrite H);
-  try reflexivity.
-  - rewrite <- IHnot_tyvar_appears_free_in_ty1.
-    rewrite <- IHnot_tyvar_appears_free_in_ty2.
-    reflexivity.
-  - rewrite <- IHnot_tyvar_appears_free_in_ty. reflexivity.
+  intros X T. split; intro H.
+  - induction T.
+    + destruct (X =? X0)%string eqn:Heq.
+      * rewrite String.eqb_eq in Heq. subst. exfalso. apply H. constructor.
+      * constructor. intro contra. subst. rewrite eqb_refl in Heq. discriminate.
+    + constructor.
+      * apply IHT1. intro contra. apply H. apply tvaf_arrow1; auto.
+      * apply IHT2. intro contra. apply H. apply tvaf_arrow2; auto.
+    + destruct (X =? X0)%string eqn:Heq.
+      * rewrite String.eqb_eq in Heq. subst. constructor.
+      * apply ntvaf_forall_free.
+        -- intro contra. subst. rewrite eqb_refl in Heq. discriminate.
+        -- apply IHT. intro contra. apply H. apply tvaf_forall; auto.
+           intro contra_eq. subst. rewrite eqb_refl in Heq. discriminate.
+    + constructor.
+  - intro contra. induction contra; inversion H; subst; auto.
 Qed.
 
-Lemma update_subst_context : forall x X S T Gamma,
-  context_ty_subst X S <{ x |-> T; Gamma }> =
-  <{ x |-> <{{[X:=S]T}}> ; (context_ty_subst X S Gamma) }> .
-Proof.
-  intros. apply functional_extensionality.
-  intro y. unfold context_ty_subst, update, t_update.
-  destruct (x0 =? y)%string; reflexivity.
-Qed.
-
-Inductive not_tyvar_appears_bounded_in_ty (X: string) : ty -> Prop :=
-| ntvab_var : forall Y,
-    not_tyvar_appears_bounded_in_ty X (TyVar Y)
-| ntvab_arrow : forall T1 T2,
-    not_tyvar_appears_bounded_in_ty X T1 ->
-    not_tyvar_appears_bounded_in_ty X T2 ->
-    not_tyvar_appears_bounded_in_ty X <{{T1 -> T2}}>
-| ntvab_forall : forall Y T1,
-    X <> Y ->
-    not_tyvar_appears_bounded_in_ty X T1 ->
-    not_tyvar_appears_bounded_in_ty X <{{-/Y, T1}}>
-| ntvab_unit :
-    not_tyvar_appears_bounded_in_ty X <{{Unit}}>
+Inductive tyvar_appears_bounded_in_ty  (X: string) : ty -> Prop :=
+  | tvab_arrow1 : forall T1 T2,
+      tyvar_appears_bounded_in_ty X T1 ->
+      tyvar_appears_bounded_in_ty X <{{T1 -> T2}}>
+  | tvab_arrow2 : forall T1 T2,
+      tyvar_appears_bounded_in_ty X T2 ->
+      tyvar_appears_bounded_in_ty X <{{T1 -> T2}}>
+  | tvab_forall_bound : forall T1,
+      tyvar_appears_bounded_in_ty X <{{-/X, T1}}>
+  | tvab_forall : forall Y T1,
+      tyvar_appears_bounded_in_ty X T1 ->
+      tyvar_appears_bounded_in_ty X <{{-/Y, T1}}>
 .
 
+Inductive not_tyvar_appears_bounded_in_ty (X: string) : ty -> Prop :=
+  | ntvab_var : forall Y,
+      not_tyvar_appears_bounded_in_ty X (TyVar Y)
+  | ntvab_arrow : forall T1 T2,
+      not_tyvar_appears_bounded_in_ty X T1 ->
+      not_tyvar_appears_bounded_in_ty X T2 ->
+      not_tyvar_appears_bounded_in_ty X <{{T1 -> T2}}>
+  | ntvab_forall : forall Y T1,
+      X <> Y ->
+      not_tyvar_appears_bounded_in_ty X T1 ->
+      not_tyvar_appears_bounded_in_ty X <{{-/Y, T1}}>
+  | ntvab_unit :
+      not_tyvar_appears_bounded_in_ty X <{{Unit}}>
+.
+
+Lemma nottvab_ntvab_iff : forall X T,
+  ~ tyvar_appears_bounded_in_ty X T <-> not_tyvar_appears_bounded_in_ty X T.
+Proof.
+  intros X T. split; intro H.
+  - induction T.
+    + constructor.
+    + constructor.
+      * apply IHT1. intro contra. apply H. apply tvab_arrow1; auto.
+      * apply IHT2. intro contra. apply H. apply tvab_arrow2; auto.
+    + destruct (X =? X0)%string eqn:Heq.
+      * rewrite String.eqb_eq in Heq. subst.
+        exfalso. apply H. constructor.
+      * apply ntvab_forall.
+        -- intro contra. subst. rewrite String.eqb_refl in Heq. discriminate.
+        -- apply IHT. intro contra. apply H. apply tvab_forall; auto.
+    + constructor.
+  - intro contra. induction contra; inversion H; subst; auto.
+Qed.
+
+Inductive tyvar_appears_free_in_term (X: string) : tm -> Prop :=
+  | tvaft_abs1 : forall x T t,
+      tyvar_appears_free_in_ty X T ->
+      tyvar_appears_free_in_term X (TmAbs x T t)
+  | tvaft_abs2 : forall x T t,
+      tyvar_appears_free_in_term X t ->
+      tyvar_appears_free_in_term X (TmAbs x T t)
+  | tvaft_app1 : forall t1 t2,
+      tyvar_appears_free_in_term X t1 ->
+      tyvar_appears_free_in_term X (TmApp t1 t2)
+  | tvaft_app2 : forall t1 t2,
+      tyvar_appears_free_in_term X t2 ->
+      tyvar_appears_free_in_term X (TmApp t1 t2)
+  | tvaft_tyabs : forall Y t,
+      X <> Y ->
+      tyvar_appears_free_in_term X t ->
+      tyvar_appears_free_in_term X (TmTyAbs Y t)
+  | tvaft_tyapp1 : forall t T,
+      tyvar_appears_free_in_term X t ->
+      tyvar_appears_free_in_term X (TmTyApp t T)
+  | tvaft_tyapp2 : forall t T,
+      tyvar_appears_free_in_ty X T ->
+      tyvar_appears_free_in_term X (TmTyApp t T).
+
+Inductive not_tyvar_appears_free_in_term (X: string) : tm -> Prop :=
+  | ntvaft_var : forall x,
+      not_tyvar_appears_free_in_term X (TmVar x)
+  | ntvaft_abs : forall x T t,
+      not_tyvar_appears_free_in_ty X T ->
+      not_tyvar_appears_free_in_term X t ->
+      not_tyvar_appears_free_in_term X (TmAbs x T t)
+  | ntvaft_app : forall t1 t2,
+      not_tyvar_appears_free_in_term X t1 ->
+      not_tyvar_appears_free_in_term X t2 ->
+      not_tyvar_appears_free_in_term X (TmApp t1 t2)
+  | ntvaft_tyabs1 : forall t,
+      not_tyvar_appears_free_in_term X (TmTyAbs X t)
+  | ntvaft_tyabs2 : forall Y t,
+      X <> Y ->
+      not_tyvar_appears_free_in_term X t ->
+      not_tyvar_appears_free_in_term X (TmTyAbs Y t)
+  | ntvaft_tyapp : forall t T,
+      not_tyvar_appears_free_in_term X t ->
+      not_tyvar_appears_free_in_ty X T ->
+      not_tyvar_appears_free_in_term X (TmTyApp t T)
+  | ntvaft_unit :
+      not_tyvar_appears_free_in_term X TmUnit.
+
+Lemma nottvaft_ntvaft_iff : forall X t,
+  ~ tyvar_appears_free_in_term X t <-> not_tyvar_appears_free_in_term X t.
+Proof.
+  intros X t. split; intro H.
+  - induction t.
+    + constructor.
+    + constructor.
+      * apply nottvaf_ntvaf_iff. intro contra. apply H. apply tvaft_abs1. assumption.
+      * apply IHt. intro contra. apply H. apply tvaft_abs2. assumption.
+    + constructor.
+      * apply IHt1. intro contra. apply H. apply tvaft_app1. assumption.
+      * apply IHt2. intro contra. apply H. apply tvaft_app2. assumption.
+    + destruct (X =? X0)%string eqn:Heq.
+      * rewrite String.eqb_eq in Heq. subst. constructor.
+      * constructor.
+        -- intro contra. subst. rewrite String.eqb_refl in Heq. discriminate.
+        -- apply IHt. intro contra. apply H. apply tvaft_tyabs; auto.
+           intro contra_eq. subst. rewrite String.eqb_refl in Heq. discriminate.
+    + constructor.
+      * apply IHt. intro contra. apply H. apply tvaft_tyapp1. assumption.
+      * apply nottvaf_ntvaf_iff. intro contra. apply H. apply tvaft_tyapp2. assumption.
+    + constructor.
+  - intro contra. induction contra; inversion H; subst; auto.
+    + apply nottvaf_ntvaf_iff in H3. apply H3. assumption.
+    + apply nottvaf_ntvaf_iff in H4. apply H4. assumption.
+Qed.
+
+Inductive tyvar_appears_bounded_in_term (X: string) : tm -> Prop :=
+  | tvabt_abs1 : forall x T t,
+      tyvar_appears_bounded_in_ty X T ->
+      tyvar_appears_bounded_in_term X (TmAbs x T t)
+  | tvabt_abs2 : forall x T t,
+      tyvar_appears_bounded_in_term X t ->
+      tyvar_appears_bounded_in_term X (TmAbs x T t)
+  | tvabt_app1 : forall t1 t2,
+      tyvar_appears_bounded_in_term X t1 ->
+      tyvar_appears_bounded_in_term X (TmApp t1 t2)
+  | tvabt_app2 : forall t1 t2,
+      tyvar_appears_bounded_in_term X t2 ->
+      tyvar_appears_bounded_in_term X (TmApp t1 t2)
+  | tvabt_tyabs : forall Y t,
+      tyvar_appears_bounded_in_term X t ->
+      tyvar_appears_bounded_in_term X (TmTyAbs Y t)
+  | tvabt_tyabs_bound : forall t,
+      tyvar_appears_bounded_in_term X (TmTyAbs X t)
+  | tvabt_tyapp1 : forall t T,
+      tyvar_appears_bounded_in_term X t ->
+      tyvar_appears_bounded_in_term X (TmTyApp t T)
+  | tvabt_tyapp2 : forall t T,
+      tyvar_appears_bounded_in_ty X T ->
+      tyvar_appears_bounded_in_term X (TmTyApp t T)
+.
 Inductive not_tyvar_appears_bounded_in_term (X: string) : tm -> Prop :=
   | ntvabt_var : forall x,
       not_tyvar_appears_bounded_in_term X (TmVar x)
@@ -449,8 +629,249 @@ Inductive not_tyvar_appears_bounded_in_term (X: string) : tm -> Prop :=
       not_tyvar_appears_bounded_in_term X TmUnit
 .
 
+Lemma nottvabt_ntvabt_iff : forall X t,
+  ~ tyvar_appears_bounded_in_term X t <-> not_tyvar_appears_bounded_in_term X t.
+Proof.
+  intros X t. split; intro H.
+  - induction t; constructor.
+    + apply IHt. intro contra. apply H. apply tvabt_abs2; auto.
+    + apply nottvab_ntvab_iff. intro contra. apply H. apply tvabt_abs1; auto.
+    + apply IHt1. intro contra. apply H. apply tvabt_app1; auto.
+    + apply IHt2. intro contra. apply H. apply tvabt_app2; auto.
+    + destruct (X =? X0)%string eqn:Heq.
+      * rewrite String.eqb_eq in Heq. subst. exfalso. apply H. apply tvabt_tyabs_bound.
+      * intro contra. subst. rewrite String.eqb_refl in Heq. discriminate.
+    + apply IHt. intro contra. apply H. apply tvabt_tyabs; auto.
+    + apply IHt. intro contra. apply H. apply tvabt_tyapp1; auto.
+    + apply nottvab_ntvab_iff. intro contra. apply H. apply tvabt_tyapp2; auto.
+  - intro contra. induction contra; inversion H; subst; auto.
+    + apply nottvab_ntvab_iff in H5. apply H5. assumption.
+    + apply nottvab_ntvab_iff in H4. apply H4. assumption.
+Qed.
+
+Definition tyvar_appears_free_in_context (X: string) (Gamma: context) :=
+  exists x T, Gamma x = Some T /\ tyvar_appears_free_in_ty X T.
+
+Definition not_tyvar_appears_free_in_context (X: string) (Gamma: context) :=
+  forall x T, Gamma x = Some T -> not_tyvar_appears_free_in_ty X T.
+
+Lemma nottvafc_ntvafc_iff : forall X Gamma, 
+  ~ tyvar_appears_free_in_context X Gamma <-> not_tyvar_appears_free_in_context X Gamma.
+Proof.
+  intros X Gamma. split; intro H.
+  - unfold not_tyvar_appears_free_in_context.
+    intros x T Hctx. apply nottvaf_ntvaf_iff.
+    intro contra. apply H. unfold tyvar_appears_free_in_context.
+    exists x, T. split; assumption.
+  - intro contra. unfold tyvar_appears_free_in_context in contra.
+    destruct contra as [x [T [Hctx Htvaf] ] ].
+    unfold not_tyvar_appears_free_in_context in H.
+    apply H in Hctx. apply nottvaf_ntvaf_iff in Hctx.
+    apply Hctx. assumption.
+Qed.
+
+Definition tyvar_appears_bounded_in_context (X: string) (Gamma: context) :=
+  exists x T, Gamma x = Some T /\ tyvar_appears_bounded_in_ty X T.
+
 Definition not_tyvar_appears_bounded_in_context (X: string) (Gamma: context) :=
-  forall x T, Gamma x = Some T -> not_tyvar_appears_bounded_in_ty X T .
+  forall x T, Gamma x = Some T -> not_tyvar_appears_bounded_in_ty X T.
+
+Lemma nottvabc_ntvabc_iff : forall X Gamma, 
+  ~ tyvar_appears_bounded_in_context X Gamma <-> not_tyvar_appears_bounded_in_context X Gamma.
+Proof.
+  intros X Gamma. split; intro H.
+  - unfold not_tyvar_appears_bounded_in_context.
+    intros x T Hctx. apply nottvab_ntvab_iff.
+    intro contra. apply H. unfold tyvar_appears_bounded_in_context.
+    exists x, T. split; assumption.
+  - intro contra. unfold tyvar_appears_bounded_in_context in contra.
+    destruct contra as [x [T [Hctx Htvab] ] ].
+    unfold not_tyvar_appears_bounded_in_context in H.
+    apply H in Hctx. apply nottvab_ntvab_iff in Hctx.
+    apply Hctx. assumption.
+Qed.
+
+Inductive tyvar_bounded_left_notfree_right : tm -> Prop :=
+  | tvblnfr_var : forall (x: string),
+      tyvar_bounded_left_notfree_right <{x}>
+  | tvblnfr_abs : forall x T1 t1,
+      tyvar_bounded_left_notfree_right t1 ->
+      tyvar_bounded_left_notfree_right <{\x:T1, t1}>
+  | tvblnfr_app : forall t1 t2,
+      tyvar_bounded_left_notfree_right t1 ->
+      tyvar_bounded_left_notfree_right t2 ->
+      tyvar_bounded_left_notfree_right <{t1 t2}>
+  | tvblnfr_tyabs : forall X t,
+      tyvar_bounded_left_notfree_right t ->
+      tyvar_bounded_left_notfree_right <{\\X, t}>
+  | tvblnfr_tyapp : forall t T,
+      ( forall X,
+        tyvar_appears_free_in_ty X T ->
+        ~ tyvar_appears_bounded_in_term X t ) ->
+      tyvar_bounded_left_notfree_right t ->
+      tyvar_bounded_left_notfree_right <{t[T]}>
+  | tvblnfr_unit :
+      tyvar_bounded_left_notfree_right <{unit}>.
+Hint Constructors tyvar_bounded_left_notfree_right : core.
+
+Inductive bounded_tyvar_unique : tm -> Prop :=
+  | btvuni_var : forall x,
+      bounded_tyvar_unique (TmVar x)
+  | btvuni_abs : forall x T t,
+      bounded_tyvar_unique t ->
+      bounded_tyvar_unique (TmAbs x T t)
+  | btvuni_app : forall t1 t2,
+      bounded_tyvar_unique t1 ->
+      bounded_tyvar_unique t2 ->
+      bounded_tyvar_unique (TmApp t1 t2)
+  | btvuni_tyabs : forall X t,
+      not_tyvar_appears_bounded_in_term X t ->
+      bounded_tyvar_unique t ->
+      bounded_tyvar_unique (TmTyAbs X t)
+  | btvuni_tyapp : forall t T,
+      bounded_tyvar_unique t ->
+      bounded_tyvar_unique (TmTyApp t T)
+  | btvuni_unit :
+      bounded_tyvar_unique TmUnit
+.
+
+Lemma weakening : forall Gamma Gamma' t T,
+     includedin Gamma Gamma' ->
+     <{ Gamma  |-- t \in T }>  ->
+     <{ Gamma' |-- t \in T }>.
+Proof.
+  intros Gamma Gamma' t T H Ht.
+  generalize dependent Gamma'.
+  induction Ht; intros; econstructor.
+  - apply H0. assumption.
+  - apply IHHt. apply includedin_update. apply H.
+  - apply IHHt1. assumption.
+  - apply IHHt2. assumption.
+  - apply IHHt. assumption.
+  - apply H.
+  - apply IHHt. assumption.
+Qed.
+
+Lemma context_invariance : forall Gamma Gamma' t T,
+     <{ Gamma |-- t \in T }> ->
+     (forall x, var_appears_free_in x t -> Gamma x = Gamma' x) ->
+     <{ Gamma' |-- t \in T }>.
+Proof.
+  intros.
+  generalize dependent Gamma'.
+  induction H as [| ? x0 ????? | | | |]; intros; auto.
+  - apply T_Var. rewrite <- H. symmetry. apply H0. apply vaf_var.
+  - apply T_Abs. apply IHhas_type. intros.
+    unfold update. unfold t_update. destruct (x0 =? x1)%string eqn:Eqx0.
+    + reflexivity.
+    + apply H0. apply vaf_abs.
+      * rewrite <- eqb_neq. apply Eqx0.
+      * apply H1.
+  - eapply T_App.
+    + apply IHhas_type1. intros. apply H1. apply vaf_app1. apply H2.
+    + apply IHhas_type2. intros. apply H1. apply vaf_app2. apply H2.
+  - constructor. apply IHhas_type. auto.
+  - apply T_TApp with (X:=X0) (T1:=T1); try assumption.
+    apply IHhas_type. auto.
+  - constructor.
+Qed.
+
+Lemma var_subst_preserves_typing : forall Gamma x U t v T,
+  ( forall y,
+      var_appears_free_in y v -> ~ var_appears_bounded_in y t) ->
+  <{ x |-> U ; Gamma |-- t \in T }> ->
+  <{ Gamma |-- v \in U }>   ->
+  <{ Gamma |-- [x:=v]t \in T }>.
+Proof.
+  intros Gamma x U t v T Hvar Ht Hv.
+  remember (x |-> U; Gamma) as Gamma'.
+  generalize dependent Gamma.
+  induction Ht; intros Gamma' G Hv; simpl; eauto.
+  - destruct (x =? x0)%string eqn: Eqx. 
+    + subst. rewrite eqb_eq in Eqx. rewrite Eqx in H.
+      unfold update in H. unfold t_update in H.
+      rewrite eqb_refl in H. inversion H.
+      rewrite <- H1; assumption. 
+    + subst. apply T_Var. unfold update in H.
+      unfold t_update in H. rewrite Eqx in H.
+      apply H. 
+  - destruct (x =? x0)%string eqn: Eqx.
+    + apply T_Abs. apply weakening with (Gamma:= <{ x0 |-> T2; Gamma }>).
+      * intros y T Hin. rewrite G in Hin. rewrite eqb_eq in Eqx.
+        rewrite Eqx in Hin. rewrite update_shadow in Hin.
+        apply Hin.
+      * apply Ht.
+    + apply T_Abs. apply IHHt.
+      * intros y' Hy'. apply Hvar in Hy'. intro Hy''.
+        rewrite notvab_nvab_iff in Hy'.
+        inversion Hy'. rewrite <- notvab_nvab_iff in H3.
+        apply H3. assumption.
+      * rewrite G. rewrite update_permute.
+        { reflexivity. }
+        { rewrite <- eqb_neq. apply Eqx. }
+      * apply context_invariance with (Gamma:=Gamma'); try assumption.
+        intros y Hy. apply Hvar in Hy .
+        rewrite notvab_nvab_iff in Hy. inversion Hy.
+        unfold update, t_update. rewrite <- eqb_neq in H1.
+        rewrite H1. reflexivity.
+  - apply T_App with T2;
+    [apply IHHt1 | apply IHHt2];
+    try assumption;
+    intros; apply Hvar in H; rewrite notvab_nvab_iff in *;
+    inversion H; assumption.
+  - constructor. apply IHHt; auto. 
+    intros y Hyf Hyb. apply Hvar in Hyf.
+    apply Hyf. constructor. assumption.
+  - apply T_TApp with (X:=X0) (T1:=T1).
+    + assumption.
+    + apply IHHt; try assumption.
+      intros y Hyf Hyb. apply Hvar in Hyf.
+      apply Hyf. constructor. assumption.
+  - apply T_Unit.
+Qed.
+
+Definition context_ty_subst X S (Gamma: context) : context :=
+    fun x =>
+      match Gamma x with
+      | Some T => Some (<{{[X:=S] T}}>)
+      | None => None
+      end.
+
+Lemma ntvaf_subst_eq_ty : forall X S T,
+  not_tyvar_appears_free_in_ty X T ->
+  T = <{{ [X:=S] T }}>.
+Proof.
+  intros X S T H.
+  induction H; simpl;
+  try rewrite eqb_refl;
+  try (apply eqb_neq in H; rewrite H);
+  try reflexivity.
+  - rewrite <- IHnot_tyvar_appears_free_in_ty1.
+    rewrite <- IHnot_tyvar_appears_free_in_ty2.
+    reflexivity.
+  - rewrite <- IHnot_tyvar_appears_free_in_ty. reflexivity.
+Qed.
+
+Lemma ntvaf_subst_eq_context : forall X S Gamma,
+  not_tyvar_appears_free_in_context X Gamma ->
+  Gamma = context_ty_subst X S Gamma.
+Proof.
+  unfold not_tyvar_appears_free_in_context, context_ty_subst.
+  intros X T Gamma H. apply functional_extensionality.
+  intros x. destruct (Gamma x) eqn: EqY.
+  - f_equal. apply ntvaf_subst_eq_ty. apply H with x. 
+    assumption.
+  - reflexivity.
+Qed.
+
+Lemma update_subst_context : forall x X S T Gamma,
+  context_ty_subst X S <{ x |-> T; Gamma }> =
+  <{ x |-> <{{[X:=S]T}}> ; (context_ty_subst X S Gamma) }> .
+Proof.
+  intros. apply functional_extensionality.
+  intro y. unfold context_ty_subst, update, t_update.
+  destruct (x0 =? y)%string; reflexivity.
+Qed.
 
 Lemma ntvab_subst_preservation : forall X Y T S,
   not_tyvar_appears_bounded_in_ty X T ->
@@ -513,7 +934,7 @@ Proof.
       apply eqb_eq in EqX. apply eqb_eq in EqY. subst.
       apply Neq. reflexivity.
     + rewrite EqY. reflexivity.
-    + rewrite EqX. apply ntvaf_subst_ty. apply H2.
+    + rewrite EqX. apply ntvaf_subst_eq_ty. apply H2.
     + rewrite EqX. rewrite EqY. reflexivity.
   - simpl. inversion H1.
     rewrite IHT1; try assumption.
@@ -530,128 +951,118 @@ Proof.
   - reflexivity.
 Qed.
 
-Lemma type_preservation_tysubst : forall Gamma Gamma' X S t T,
-  <{ Gamma |-- t \in T }> ->
+Ltac IH_solve IH Htvblnfr :=
+  apply IH; try reflexivity;
+  try (intros _Y _HY; apply Htvblnfr in _HY as [_HYt _HYG];
+      inversion _HYt; split); 
+  assumption.
+
+Lemma tysubst_preserves_typing : forall Gamma Gamma' X S t T,
   not_tyvar_appears_bounded_in_context X Gamma ->
   not_tyvar_appears_bounded_in_term X t ->
-  closed S ->
+  ( forall Y,
+      tyvar_appears_free_in_ty Y S ->
+      not_tyvar_appears_bounded_in_term Y t /\ not_tyvar_appears_bounded_in_context Y Gamma )->
+  <{ Gamma |-- t \in T }> ->
   Gamma' = context_ty_subst X S Gamma ->
   <{ Gamma' |-- [[X:=S]]t \in [X:=S]T }>.
 Proof.
-  intros Gamma Gamma' X S t T H.
+  intros Gamma Gamma' X S t T Hntabc Hntabt Htvblnfr H.
   generalize dependent Gamma'.
-  induction H; simpl; intros; subst.
+  induction H; simpl; intros;
+  inversion Hntabt; subst.
   - apply T_Var. unfold context_ty_subst in *.
     destruct (Gamma x0).
     + f_equal. injection H as H'. rewrite H'. reflexivity.
     + discriminate.
   - apply T_Abs. rewrite <- update_subst_context.
-    apply IHhas_type.
-    + unfold not_tyvar_appears_bounded_in_context.
-      unfold update, t_update. intros y T subH.
-      destruct (x0 =? y)%string.
-      * inversion subH. inversion H1. subst. assumption.
-      * unfold not_tyvar_appears_bounded_in_context in H0.
-        apply H0 with y. assumption.
-    + inversion H1. assumption.
-    + assumption. 
-    + reflexivity.
+    apply IHhas_type; try reflexivity; try assumption.
+    + unfold not_tyvar_appears_bounded_in_context in *.
+      unfold update, t_update. intros.
+      destruct (x0=?x1)%string.
+      * inversion H0. subst. assumption.
+      * apply Hntabc with x1. assumption.
+    + intros Y HY. apply Htvblnfr in HY as [HYt HYG]. split.
+      * inversion HYt. assumption.
+      * intros x T Hx. unfold update, t_update in Hx.
+        destruct (x0=?x)%string.
+        { inversion Hx. subst. inversion HYt. assumption. }
+        { apply HYG in Hx. assumption. }
   - eapply T_App.
-    + apply IHhas_type1;
-      try reflexivity; inversion H2; assumption.
-    + apply IHhas_type2;
-      try reflexivity; inversion H2; assumption.
-  - inversion H1. apply eqb_neq in H5. rewrite H5. apply T_TAbs.
-    apply IHhas_type; try reflexivity; assumption.
-  - inversion H2.
-    apply ntvab_typing with (X:=X) in H0; try assumption.
-    inversion H0. 
-    apply T_TApp with (X:=X0) (T1:=<{{[X:=S]T1}}>).
+    + IH_solve IHhas_type1 Htvblnfr.
+    + IH_solve IHhas_type2 Htvblnfr.
+  - apply eqb_neq in H3. rewrite H3. apply T_TAbs.
+    IH_solve IHhas_type Htvblnfr.
+  - apply ntvab_typing with (X:=X) in H0 as HT; try assumption.
+    inversion HT.
+    apply T_TApp with (X:=X0) (S:=<{{[X:=S]S0}}>)
+    (T1:=<{{[X:=S]T1}}>) (T1':=<{{[X:=S]([X0:=S0]T1)}}>).
     + apply ty_subst_distribution; try assumption.
-      * apply H3. 
-    + apply eqb_neq in H9. 
-      simpl in IHhas_type. rewrite H9 in IHhas_type. 
-      apply IHhas_type;
-      try reflexivity; inversion H2; assumption.
-    - apply T_Unit.
+      apply nottvaf_ntvaf_iff. intro HX0S.
+      apply Htvblnfr in HX0S as [Ht HG].
+      inversion Ht.
+      specialize (ntvab_typing _ _ _ _ HG H8 H0) as contra.
+      apply nottvab_ntvab_iff in contra. apply contra. constructor.
+    + apply eqb_neq in H2. simpl in IHhas_type. rewrite H2 in IHhas_type.
+      IH_solve IHhas_type Htvblnfr.
+  - apply T_Unit.
 Qed.
 
-Inductive bounded_tyvar_unique : tm -> Prop :=
-  | btvuni_var : forall x,
-      bounded_tyvar_unique (TmVar x)
-  | btvuni_abs : forall x T t,
-      bounded_tyvar_unique t ->
-      bounded_tyvar_unique (TmAbs x T t)
-  | btvuni_app : forall t1 t2,
-      bounded_tyvar_unique t1 ->
-      bounded_tyvar_unique t2 ->
-      bounded_tyvar_unique (TmApp t1 t2)
-  | btvuni_tyabs : forall X t,
-      not_tyvar_appears_bounded_in_term X t ->
-      bounded_tyvar_unique t ->
-      bounded_tyvar_unique (TmTyAbs X t)
-  | btvuni_tyapp : forall t T,
-      bounded_tyvar_unique t ->
-      bounded_tyvar_unique (TmTyApp t T)
-  | btvuni_unit :
-      bounded_tyvar_unique TmUnit
-.
+Ltac IH_solve_2 IH Htvb Ctvabt Htvf1 Ctvaft Htvf2 :=
+  apply IH; try reflexivity; try assumption;
+  try (intros; apply Htvb; apply Ctvabt; assumption);
+  try (intros; apply Htvf1; apply Ctvaft; assumption);
+  try (intros _X _H; apply Htvf2 in _H; inversion _H; assumption).
 
-Inductive applied_type_is_closed : tm -> Prop :=
-  | atic_var : forall x,
-      applied_type_is_closed (TmVar x)
-  | atic_abs : forall x T t,
-      applied_type_is_closed t ->
-      applied_type_is_closed (TmAbs x T t)
-  | atic_app : forall t1 t2,
-      applied_type_is_closed t1 ->
-      applied_type_is_closed t2 ->
-      applied_type_is_closed (TmApp t1 t2)
-  | atic_tyabs : forall X t,
-      applied_type_is_closed t ->
-      applied_type_is_closed (TmTyAbs X t)
-  | atic_tyapp : forall t T,
-      applied_type_is_closed t ->
-      closed T ->
-      applied_type_is_closed (TmTyApp t T)
-  | atic_unit :
-      applied_type_is_closed TmUnit
-.
-
-Theorem type_preservation: forall t t' T,
+Theorem type_preservation: forall Gamma t t' T,
+  var_bounded_left_notfree_right t ->
+  tyvar_bounded_left_notfree_right t ->
   bounded_tyvar_unique t ->
-  applied_type_is_closed t ->
-  <{ empty |-- t \in T }> ->
+  ( forall X,
+      tyvar_appears_bounded_in_term X t ->
+      not_tyvar_appears_bounded_in_context X Gamma ) ->
+  ( forall X,
+      tyvar_appears_free_in_term X t ->
+      not_tyvar_appears_bounded_in_context X Gamma ) ->
+  ( forall X,
+      tyvar_appears_free_in_context X Gamma ->
+      not_tyvar_appears_bounded_in_term X t ) ->
+  <{ Gamma |-- t \in T }> ->
   t --> t' ->
-  <{ empty |-- t' \in T }>.
+  <{ Gamma |-- t' \in T }>.
 Proof.
-  intros t t' T Hbounded Hclosed HT.
+  intros Gamma t t' T Hvblnr Htvblnr Hbtvu Htvb Htvf1 Htvf2 HT.
   generalize dependent t'.
-  remember empty as Gamma.
   induction HT;
-  intros t' HSt; inversion HSt; subst.
+  intros t' HSt; inversion HSt;
+  inversion Hvblnr; inversion Htvblnr; inversion Hbtvu;
+  subst.
   - inversion HT1. subst.
-    apply type_preservation_subst with (S:=T2).
-    * apply H1.
-    * apply HT2.
+    apply var_subst_preserves_typing with (U:=T2); try assumption.
+    * intros y Hfy Hby. apply H5 in Hfy.
+      apply Hfy. destruct (y=?x0)%string eqn: Eqy.
+      { apply eqb_eq in Eqy. subst y. constructor. }
+      { rewrite eqb_sym in Eqy. apply eqb_neq in Eqy. constructor;
+        assumption. }
+  - apply T_App with T2; try assumption. 
+    IH_solve_2 IHHT1 Htvb tvabt_app1 Htvf1 tvaft_app1 Htvf2.
   - apply T_App with T2; try assumption.
-    inversion Hbounded. inversion Hclosed.
-    apply IHHT1; try reflexivity; assumption.
-  - apply T_App with T2; try assumption.
-    inversion Hbounded. inversion Hclosed.
-    apply IHHT2; try reflexivity; assumption.
+    IH_solve_2 IHHT2 Htvb tvabt_app2 Htvf1 tvaft_app2 Htvf2.
   - eapply T_TApp.  
     * reflexivity.
-    * inversion Hbounded. inversion Hclosed.
-    apply IHHT; try reflexivity; assumption.
-  - inversion HT.
-    apply type_preservation_tysubst with empty.
+    * IH_solve_2 IHHT Htvb tvabt_tyapp1 Htvf1 tvaft_tyapp1 Htvf2.
+  - inversion HT. subst.
+    apply tysubst_preserves_typing with Gamma.
+    + apply Htvb. constructor. apply tvabt_tyabs_bound.
+    + inversion H11. assumption.
+    + intros. split.
+      * apply H8 in H. rewrite nottvabt_ntvabt_iff in H.
+        inversion H. assumption.
+      * apply Htvf1. apply tvaft_tyapp2. assumption.
     + assumption.
-    + unfold not_tyvar_appears_bounded_in_context.
-      intros. discriminate.
-    + inversion Hbounded. inversion H6. subst. assumption.
-    + inversion Hclosed. assumption.
-    + apply functional_extensionality.
-      unfold context_ty_subst. reflexivity.
+    + assert (HG: not_tyvar_appears_free_in_context X0 Gamma).
+      { apply nottvafc_ntvafc_iff. intros H. apply Htvf2 in H.
+        apply nottvabt_ntvabt_iff in H. apply H. apply tvabt_tyapp1.
+        apply tvabt_tyabs_bound. }
+      apply ntvaf_subst_eq_context. assumption.
 Qed.
- 
